Formalized the UTF-8 encoding

hol.ml
@@ -100,8 +100,8 @@ loads "fusion.ml";;
 loads "opentheory/logging.ml";;
 
 (* Uncomment to extract the standard theory library
-start_logging ();;
 *)
+start_logging ();;
 
 (* ------------------------------------------------------------------------- *)
 (* Some extra support stuff needed outside the core.                         *)
@@ -175,5 +175,5 @@ loads "database.ml";;   (* List of name-theorem pairs for search system      *)
 loads "opentheory/stdlib/all.ml";;
 
 (* Uncomment to extract the standard theory library
-stop_logging ();;
 *)
+stop_logging ();;
