opentheory/stdlib/all.ml
@@ -1,41 +1,6 @@
 (* ------------------------------------------------------------------------- *)
-(* Additions to the standard library.                                        *)
+(* Additions to the OpenTheory standard library.                             *)
 (* ------------------------------------------------------------------------- *)
 
-logfile "option-thm";;
-
-let option_distinct = distinctness "option";;
-
-export_thm option_distinct;;
-
-let option_inj = injectivity "option";;
-
-export_thm option_inj;;
-
-let option_cases = prove_cases_thm option_INDUCT;;
-
-export_thm option_cases;;
-
-logfile "option-case";;
-
-let case_option_def = new_recursive_definition option_RECURSION
-  `(case_option f b NONE = (b:B)) /\
-   (case_option f b (SOME a) = f (a:A))`;;
-
-export_thm case_option_def;;
-
-logfile "list-thm";;
-
-let list_cases = prove_cases_thm list_INDUCT;;
-
-export_thm list_cases;;
-
-logfile "list-case";;
-
-let case_list_def = new_recursive_definition list_RECURSION
-  `(case_list f b [] = (b:B)) /\
-   (case_list f b (CONS h t) = f (h:A) t)`;;
-
-export_thm case_list_def;;
-
-logfile_end ();;
+loads "opentheory/stdlib/option.ml";;
+loads "opentheory/stdlib/list.ml";;
