opentheory/examples/word.ml
@@ -2,58 +2,6 @@
 (* A functor theory of words.                                                *)
 (* ------------------------------------------------------------------------- *)
 
-logfile "list-interval-def";;
-
-let interval_def = new_recursive_definition num_RECURSION
-  `(!m. interval m 0 = []) /\
-   (!m n. interval m (SUC n) = CONS m (interval (SUC m) n))`;;
-
-export_thm interval_def;;
-
-logfile "list-interval-thm";;
-
-let length_interval = prove
-  (`!m n. LENGTH (interval m n) = n`,
-   ONCE_REWRITE_TAC [SWAP_FORALL_THM] THEN
-   MATCH_MP_TAC num_INDUCTION THEN
-   SIMP_TAC [LENGTH; interval_def; SUC_INJ]);;
-
-export_thm length_interval;;
-
-logfile "list-zipwith-def";;
-
-let zipwith_raw_def = new_recursive_definition list_RECURSION
-  `(!f l. zipwith f [] l = []) /\
-   (!f h t l.
-      zipwith f (CONS h t) l =
-      CONS (f h (HD l)) (zipwith f t (TL l)))`;;
-
-let zipwith_def = prove
-   (`(!f. zipwith (f : A -> B -> C) [] [] = []) /\
-     (!f h1 h2 t1 t2.
-        zipwith (f : A -> B -> C) (CONS h1 t1) (CONS h2 t2) =
-        CONS (f h1 h2) (zipwith f t1 t2))`,
-    REWRITE_TAC [zipwith_raw_def; HD; TL]);;
-
-export_thm zipwith_def;;
-
-logfile "list-zipwith-thm";;
-
-let length_zipwith = prove
-  (`!(f : A -> B -> C) l1 l2 n.
-      LENGTH l1 = n /\ LENGTH l2 = n ==> LENGTH (zipwith f l1 l2) = n`,
-   GEN_TAC THEN
-   LIST_INDUCT_TAC THEN
-   LIST_INDUCT_TAC THEN
-   ASM_SIMP_TAC [LENGTH; zipwith_def] THEN
-   GEN_TAC THEN
-   MP_TAC (SPEC `n:num` num_CASES) THEN
-   STRIP_TAC THEN
-   ASM_SIMP_TAC [NOT_SUC; SUC_INJ] THEN
-   FIRST_ASSUM MATCH_ACCEPT_TAC);;
-
-export_thm length_zipwith;;
-
 new_constant ("word_width", `:num`);;
 
 logfile "word-def";;
