opentheory/examples/char.ml
@@ -76,6 +76,172 @@ export_thm unicode_tybij;;
 
 logfile "char-utf8";;
 
-(* decode : byte list -> (char * byte list) option *)
+let is_cont_def = new_definition
+  `!b. is_cont b <=> byte_bit b 7 /\ ~byte_bit b 6`;;
+
+export_thm is_cont_def;;
+
+let parse_cont_def = new_definition
+  `parse_cont = parse_some is_cont`;;
+
+export_thm parse_cont_def;;
+
+let parse_cont2_def = new_definition
+  `parse_cont2 = parse_pair parse_cont parse_cont`;;
+
+export_thm parse_cont2_def;;
+
+let parse_cont3_def = new_definition
+  `parse_cont3 = parse_pair parse_cont parse_cont2`;;
+
+export_thm parse_cont3_def;;
+
+let decoder_parse_def = new_definition
+  `!b0 s.
+     decoder_parse b0 s =
+     if byte_bit b0 7 then
+       if byte_bit b0 6 then
+         if byte_bit b0 5 then
+           if byte_bit b0 4 then
+             if byte_bit b0 3 then
+               NONE
+             else
+               case_option
+                 NONE
+                 (\ ((b1,(b2,b3)),s').
+                    let w = byte_shl (byte_and b0 (num_to_byte 7)) 2 in
+                    let z = byte_shr (byte_and b1 (num_to_byte 48)) 4 in
+                    let p = byte_or w z in
+                    if p = num_to_byte 0 \/ byte_lt (num_to_byte 16) p then
+                      NONE
+                    else
+                      let pl = mk_plane p in
+                      let z0 = byte_shl (byte_and b1 (num_to_byte 15)) 4 in
+                      let y0 = byte_shr (byte_and b2 (num_to_byte 60)) 2 in
+                      let p0 = byte_or z0 y0 in
+                      let y1 = byte_shl (byte_and b2 (num_to_byte 3)) 6 in
+                      let x1 = byte_and b3 (num_to_byte 63) in
+                      let p1 = byte_or y1 x1 in
+                      let pos = mk_position (bytes_to_word16 p0 p1) in
+                      let ch = mk_unicode (pl,pos) in
+                      SOME (ch,s'))
+                 (parse parse_cont3 s)
+           else
+             case_option
+               NONE
+               (\ ((b1,b2),s').
+                  let z0 = byte_shl (byte_and b0 (num_to_byte 15)) 4 in
+                  let y0 = byte_shr (byte_and b1 (num_to_byte 60)) 2 in
+                  let p0 = byte_or z0 y0 in
+                  if byte_lt p0 (num_to_byte 8) \/
+                     (byte_le (num_to_byte 216) p0 /\
+                      byte_le p0 (num_to_byte 223)) then
+                    NONE
+                  else
+                    let y1 = byte_shl (byte_and b1 (num_to_byte 3)) 6 in
+                    let x1 = byte_and b2 (num_to_byte 63) in
+                    let p1 = byte_or y1 x1 in
+                    if p0 = num_to_byte 255 /\ byte_le (num_to_byte 254) p1 then
+                      NONE
+                    else
+                      let pl = mk_plane (num_to_byte 0) in
+                      let pos = mk_position (bytes_to_word16 p0 p1) in
+                      let ch = mk_unicode (pl,pos) in
+                      SOME (ch,s'))
+               (parse parse_cont2 s)
+         else
+           case_option
+             NONE
+             (\ (b1,s').
+               let pl = mk_plane (num_to_byte 0) in
+               let p0 = byte_shr (byte_and b0 (num_to_byte 28)) 2 in
+               let y1 = byte_shl (byte_and b0 (num_to_byte 3)) 6 in
+               let x1 = byte_and b1 (num_to_byte 63) in
+               let p1 = byte_or y1 x1 in
+               if p0 = num_to_byte 0 /\ byte_lt p1 (num_to_byte 128) then
+                 NONE
+               else
+                 let pos = mk_position (bytes_to_word16 p0 p1) in
+                 let ch = mk_unicode (pl,pos) in
+                 SOME (ch,s'))
+             (parse parse_cont s)
+       else
+         NONE
+     else
+       let pl = mk_plane (num_to_byte 0) in
+       let pos = mk_position (bytes_to_word16 (num_to_byte 0) b0) in
+       let ch = mk_unicode (pl,pos) in
+       SOME (ch,s)`;;
+
+export_thm decoder_parse_def;;
+
+let decoder_def = new_definition
+  `decoder = mk_parser decoder_parse`;;
+
+export_thm decoder_def;;
+
+let decode_stream_def = new_definition
+  `decode_stream = parse_stream decoder`;;
+
+export_thm decode_stream_def;;
+
+let decode_def = new_definition
+  `!bs. decode bs = stream_to_list (decode_stream (list_to_stream bs))`;;
+
+export_thm decode_def;;
+
+let encoder_def = new_definition
+  `!ch.
+     encoder ch =
+     let (pl,pos) = dest_unicode ch in
+     let p = dest_plane pl in
+     let (p0,p1) = word16_to_bytes (dest_position pos) in
+     if p = num_to_byte 0 then
+       if p0 = num_to_byte 0 then
+         if byte_bit p1 7 then
+           let b00 = byte_shr (byte_and p1 (num_to_byte 192)) 6 in
+           let b0 = byte_or (num_to_byte 192) b00 in
+           let b10 = byte_and p1 (num_to_byte 63) in
+           let b1 = byte_or (num_to_byte 128) b10 in
+           CONS b0 (CONS b1 [])
+         else
+           let b0 = p1 in
+           CONS b0 []
+       else
+         if byte_and (num_to_byte 248) p0 = num_to_byte 0 then
+           let b00 = byte_shl p0 2 in
+           let b01 = byte_shr (byte_and p1 (num_to_byte 192)) 6 in
+           let b0 = byte_or (num_to_byte 192) (byte_or b00 b01) in
+           let b10 = byte_and p1 (num_to_byte 63) in
+           let b1 = byte_or (num_to_byte 128) b10 in
+           CONS b0 (CONS b1 [])
+         else
+           let b00 = byte_shr (byte_and p0 (num_to_byte 240)) 4 in
+           let b0 = byte_or (num_to_byte 224) b00 in
+           let b10 = byte_shl (byte_and p0 (num_to_byte 15)) 2 in
+           let b11 = byte_shr (byte_and p1 (num_to_byte 192)) 6 in
+           let b1 = byte_or (num_to_byte 128) (byte_or b10 b11) in
+           let b20 = byte_and p1 (num_to_byte 63) in
+           let b2 = byte_or (num_to_byte 128) b20 in
+           CONS b0 (CONS b1 (CONS b2 []))
+     else
+       let b00 = byte_shr (byte_and p (num_to_byte 28)) 2 in
+       let b0 = byte_or (num_to_byte 240) b00 in
+       let b10 = byte_shl (byte_and p (num_to_byte 3)) 4 in
+       let b11 = byte_shr (byte_and p0 (num_to_byte 240)) 4 in
+       let b1 = byte_or (num_to_byte 128) (byte_or b10 b11) in
+       let b20 = byte_shl (byte_and p0 (num_to_byte 15)) 2 in
+       let b21 = byte_shr (byte_and p1 (num_to_byte 192)) 6 in
+       let b2 = byte_or (num_to_byte 128) (byte_or b20 b21) in
+       let b30 = byte_and p1 (num_to_byte 63) in
+       let b3 = byte_or (num_to_byte 128) b30 in
+       CONS b0 (CONS b1 (CONS b2 (CONS b3 [])))`;;
+
+export_thm encoder_def;;
+
+let encode_def = new_definition
+  `!chs. encode chs = concat (MAP encoder chs)`;;
+
+export_thm encode_def;;
 
 logfile_end ();;
