opentheory/stdlib/list.ml
@@ -1,0 +1,105 @@
+(* ------------------------------------------------------------------------- *)
+(* Additions to the standard list theory.                                    *)
+(* ------------------------------------------------------------------------- *)
+
+logfile "list-thm";;
+
+let list_cases = prove_cases_thm list_INDUCT;;
+
+export_thm list_cases;;
+
+logfile "list-dest-thm";;
+
+let NULL_EQ_NIL = prove
+ (`!l. NULL (l : A list) <=> l = []`,
+  LIST_INDUCT_TAC THEN
+  ASM_REWRITE_TAC [NULL; NOT_CONS_NIL]);;
+
+export_thm NULL_EQ_NIL;;
+
+logfile "list-case";;
+
+let case_list_def = new_recursive_definition list_RECURSION
+  `(!b f. case_list b f [] = (b:B)) /\
+   (!b f h t. case_list b f (CONS h t) = f (h:A) t)`;;
+
+export_thm case_list_def;;
+
+logfile "list-append-thm";;
+
+let NULL_APPEND = prove
+ (`!l m. NULL (APPEND (l : A list) m) <=> NULL l /\ NULL m`,
+  ASM_REWRITE_TAC [NULL_EQ_NIL; APPEND_EQ_NIL]);;
+
+export_thm NULL_APPEND;;
+
+logfile_end ();;
+
+logfile "list-concat-def";;
+
+let concat_def = new_recursive_definition list_RECURSION
+  `(concat [] = ([] : A list)) /\
+   (!h t. concat (CONS h t) = APPEND h (concat t))`;;
+
+export_thm concat_def;;
+
+logfile "list-concat-thm";;
+
+let null_concat = prove
+  (`!l. NULL (concat l) <=> ALL NULL l`,
+   LIST_INDUCT_TAC THEN
+   ASM_REWRITE_TAC [concat_def; ALL; NULL; NULL_APPEND]);;
+
+export_thm null_concat;;
+
+logfile "list-interval-def";;
+
+let interval_def = new_recursive_definition num_RECURSION
+  `(!m. interval m 0 = []) /\
+   (!m n. interval m (SUC n) = CONS m (interval (SUC m) n))`;;
+
+export_thm interval_def;;
+
+logfile "list-interval-thm";;
+
+let length_interval = prove
+  (`!m n. LENGTH (interval m n) = n`,
+   ONCE_REWRITE_TAC [SWAP_FORALL_THM] THEN
+   MATCH_MP_TAC num_INDUCTION THEN
+   SIMP_TAC [LENGTH; interval_def; SUC_INJ]);;
+
+export_thm length_interval;;
+
+logfile "list-zipwith-def";;
+
+let zipwith_raw_def = new_recursive_definition list_RECURSION
+  `(!f l. zipwith f [] l = []) /\
+   (!f h t l.
+      zipwith f (CONS h t) l =
+      CONS (f h (HD l)) (zipwith f t (TL l)))`;;
+
+let zipwith_def = prove
+   (`(!f. zipwith (f : A -> B -> C) [] [] = []) /\
+     (!f h1 h2 t1 t2.
+        zipwith (f : A -> B -> C) (CONS h1 t1) (CONS h2 t2) =
+        CONS (f h1 h2) (zipwith f t1 t2))`,
+    REWRITE_TAC [zipwith_raw_def; HD; TL]);;
+
+export_thm zipwith_def;;
+
+logfile "list-zipwith-thm";;
+
+let length_zipwith = prove
+  (`!(f : A -> B -> C) l1 l2 n.
+      LENGTH l1 = n /\ LENGTH l2 = n ==> LENGTH (zipwith f l1 l2) = n`,
+   GEN_TAC THEN
+   LIST_INDUCT_TAC THEN
+   LIST_INDUCT_TAC THEN
+   ASM_SIMP_TAC [LENGTH; zipwith_def] THEN
+   GEN_TAC THEN
+   MP_TAC (SPEC `n:num` num_CASES) THEN
+   STRIP_TAC THEN
+   ASM_SIMP_TAC [NOT_SUC; SUC_INJ] THEN
+   FIRST_ASSUM MATCH_ACCEPT_TAC);;
+
+export_thm length_zipwith;;
