opentheory/stdlib/option.ml
@@ -1,0 +1,27 @@
+(* ------------------------------------------------------------------------- *)
+(* Additions to the standard option theory.                                  *)
+(* ------------------------------------------------------------------------- *)
+
+logfile "option-thm";;
+
+let option_distinct = distinctness "option";;
+
+export_thm option_distinct;;
+
+let option_inj = injectivity "option";;
+
+export_thm option_inj;;
+
+let option_cases = prove_cases_thm option_INDUCT;;
+
+export_thm option_cases;;
+
+logfile "option-case";;
+
+let case_option_def = new_recursive_definition option_RECURSION
+  `(!b f. case_option b f NONE = (b:B)) /\
+   (!b f a. case_option b f (SOME a) = f (a:A))`;;
+
+export_thm case_option_def;;
+
+logfile_end ();;
